% This file is included by both the web and print versions of the blueprint
% via an import statment in blueprint/scr/content.tex 

\section{Local identities in semigroups}

Throughout, let \(S\) be a semigroup with associative multiplication, written multiplicatively.

\begin{definition}[Left/right/two-sided identities]
\label{def:identities}
Let \(e\in S\).
\begin{itemize}
  \item \(e\) is a \emph{left identity} if for all \(s\in S\), \(e s = s\).
  \item \(e\) is a \emph{right identity} if for all \(s\in S\), \(s e = s\).
  \item \(e\) is an \emph{identity} (two-sided) if it is both a left and a right identity; equivalently, for all \(s\in S\), \(e s = s = s e\).
\end{itemize}
\end{definition}

\begin{lemma}[Idempotence of one-sided identities]
\label{lem:identity-idempotent}
Let \(e\in S\).
\begin{itemize}
  \item If \(e\) is a left identity, then \(e e = e\).
  \item If \(e\) is a right identity, then \(e e = e\).
\end{itemize}
\uses{def:identities}
\end{lemma}
\begin{proof}
For a left identity, apply the defining property to \(s:=e\) to get \(e e = e\).
For a right identity, apply the defining property to \(s:=e\) to get \(e e = e\).
\end{proof}

\begin{lemma}[Simplification lemma]
\label{lem:simplification}
Let \(s\in S\) and let \(e,f\in S\) be idempotents. If \(s = e s f\), then \(e s = s = s f\).
\end{lemma}
\begin{proof}
Assume \(s = e s f\). Then
\[
e s \;=\; e(e s f) \;=\; (e e) s f \;=\; e s f \;=\; s,
\]
using associativity and \(e^2 = e\). Similarly,
\[
s f \;=\; (e s f) f \;=\; e s (f f) \;=\; e s f \;=\; s,
\]
using associativity and \(f^2 = f\).
\end{proof}